Move more Lemmas to HSem

Launchbury/HSem.thy
@@ -42,6 +42,10 @@ definition HSem :: "('var \<times> 'exp) list \<Rightarrow> 'var f\<rightharpoon
       (\<lambda> \<rho>'. \<rho>\<^bsub>[fdom \<rho> \<union> heapVars h]\<^esub> \<squnion> heapToEnv h (\<lambda>e. ESem e \<rho>')\<^bsub>[fdom \<rho> \<union> heapVars h]\<^esub>)
     else (\<rho>\<^bsub>[fdom \<rho> \<union> heapVars h]\<^esub>))"
 
+abbreviation HSem_syn ("\<lbrace>_\<rbrace>_"  [60,60] 60) where "\<lbrace>\<Gamma>\<rbrace>\<rho> \<equiv> HSem \<Gamma> \<rho>"
+
+abbreviation HSem_fempty  ("\<lbrace>_\<rbrace>"  [60] 60) where "\<lbrace>\<Gamma>\<rbrace> \<equiv> \<lbrace>\<Gamma>\<rbrace>fempty"
+
 text {*
 Given the predcondition hold, we can unfold the definition directly.
 *}
@@ -919,6 +923,153 @@ subsubsection {* The heap semantics can also be defined inductively over the hea
     apply (rule fix_on_least_below[OF fix_on_cond_fempty _ assms])
     using assms by (metis (full_types) fmap_below_dom heapToEnv_fdom mem_Collect_eq)
 
+  lemmas the_lookup_HSem_fempty = the_lookup_HSem_heap[OF fempty_is_HSem_cond, simp]
+
+end
+
+locale has_ignore_fresh_ESem = has_cont_ESem +
+  assumes ESem_ignores_fresh: "\<rho>1 \<le> \<rho>2 \<Longrightarrow> atom ` (fdom \<rho>2 - fdom \<rho>1) \<sharp>* e \<Longrightarrow> ESem e \<rho>1 = ESem e \<rho>2"
+begin
+
+subsubsection {* Binding more variables increases knowledge *}
+
+  lemma HSem_subset_below:
+    assumes cond2: "HSem_cond' (\<Delta>@\<Gamma>) \<rho>"
+    assumes fresh: "atom ` heapVars \<Gamma> \<sharp>* (\<Delta>, \<rho>)" 
+    shows "(\<lbrace>\<Delta>\<rbrace>\<rho>)\<^bsub>[fdom \<rho> \<union> heapVars \<Delta> \<union> heapVars \<Gamma>]\<^esub> \<sqsubseteq> \<lbrace>\<Delta>@\<Gamma>\<rbrace>\<rho>"
+  proof-
+    have fdoms: "fdom \<rho> \<union> (heapVars \<Delta> \<union> heapVars \<Gamma>) - (fdom \<rho> \<union> heapVars \<Delta>) = heapVars \<Gamma>"
+      using fresh by (auto dest: fresh_heapVars_distinct simp add: sharp_star_Env' fresh_star_Pair)
+    
+    have below: "\<lbrace>\<Delta>\<rbrace>\<rho> \<sqsubseteq> (\<lbrace>\<Delta>@\<Gamma>\<rbrace>\<rho>)\<^bsub>[fdom \<rho> \<union> heapVars \<Delta>]\<^esub>" (is "_ \<sqsubseteq> ?RHS")
+    proof (rule HSem_below)
+      show "\<rho>\<^bsub>[fdom \<rho> \<union> heapVars \<Delta>]\<^esub> \<sqsubseteq> ?RHS"
+      proof (rule fmap_expand_belowI)
+        fix x
+        assume "x \<in> fdom \<rho>"
+        with fmap_belowE[OF HSem_refines[OF cond2], where x = x]
+        show "\<rho> f! x \<sqsubseteq> ?RHS f! x" by simp
+      qed simp
+    next
+    case (goal2 x)[simp]
+      have "ESem (the (map_of \<Delta> x)) ?RHS = ESem (the (map_of \<Delta> x)) (\<lbrace>\<Delta>@\<Gamma>\<rbrace>\<rho>)"
+        apply (rule ESem_ignores_fresh[OF fmap_expand_less])
+        apply simp
+        apply auto[1]
+        apply (simp add: fdoms)
+        using fresh apply (metis fresh fresh_PairD(1) fresh_heap_expr'[OF _ the_map_of_snd[OF goal2]] fresh_star_def)
+        done
+      also have "\<dots> = ESem (the (map_of (\<Delta>@\<Gamma>) x)) (\<lbrace>\<Delta>@\<Gamma>\<rbrace>\<rho>)"
+        by (simp add: map_add_dom_app_simps)
+      also have "\<dots> \<sqsubseteq> ?RHS f! x"
+        by (simp, rule HSem_heap_below[OF cond2, where x = x, simplified])
+      finally
+      show ?case.
+    qed
+  
+    show ?thesis
+    proof(rule fmap_expand_belowI)
+    case (goal2 x) 
+      with fmap_belowE[OF below, where x = x]
+      show ?case by (cases "x\<in> fdom \<rho>", auto)
+    qed auto
+  qed
+
+  subsubsection {* Additional, fresh bindings in one or two steps *}  
+
+  lemma HSem_merge:
+    assumes distinct1: "distinctVars (\<Delta> @ \<Gamma>)"
+    assumes fresh: "atom ` heapVars \<Gamma> \<sharp>* (\<Delta>, \<rho>)"
+    assumes rho_fresh: "fdom \<rho> \<inter> heapVars (\<Gamma> @ \<Delta>) = {}"
+    shows "\<lbrace>\<Gamma>\<rbrace>\<lbrace>\<Delta>\<rbrace>\<rho> = \<lbrace>\<Gamma>@\<Delta>\<rbrace>\<rho>"
+  proof(rule below_antisym)
+    from distinct1
+    have distinct2: "distinctVars (\<Gamma> @ \<Delta>)"
+      by (auto simp add: distinctVars_append)
+  
+    from fresh
+    have Gamma_fresh: "heapVars \<Gamma> \<inter> (fdom \<rho> \<union> heapVars \<Delta>) = {}"
+      by (auto dest: fresh_heapVars_distinct simp add: sharp_star_Env' fresh_star_Pair)
+    hence fdoms: "fdom \<rho> \<union> heapVars \<Delta> \<union> heapVars \<Gamma> - (fdom \<rho> \<union> heapVars \<Delta>) = heapVars \<Gamma>"
+      by auto
+  
+    have cond1: "HSem_cond' \<Gamma> (\<lbrace>\<Delta>\<rbrace>\<rho>)"
+      apply (rule disjoint_is_HSem_cond)
+      using Gamma_fresh by auto
+    have cond2: "HSem_cond' (\<Gamma>@\<Delta>) \<rho>"
+      apply (rule disjoint_is_HSem_cond)
+      using rho_fresh by auto
+    have cond2': "HSem_cond' (\<Delta>@\<Gamma>) \<rho>"
+      apply (rule disjoint_is_HSem_cond)
+      using rho_fresh by auto
+    have cond3: "HSem_cond' \<Delta> \<rho>"
+      apply (rule disjoint_is_HSem_cond)
+      using rho_fresh by auto
+  
+    show "\<lbrace>\<Gamma>\<rbrace>\<lbrace>\<Delta>\<rbrace>\<rho> \<sqsubseteq> \<lbrace>\<Gamma>@\<Delta>\<rbrace>\<rho>"
+    proof(rule HSem_below)
+      have "(\<lbrace>\<Delta>\<rbrace>\<rho>)\<^bsub>[fdom \<rho> \<union> heapVars \<Delta> \<union> heapVars \<Gamma>]\<^esub> \<sqsubseteq> \<lbrace>\<Delta> @ \<Gamma>\<rbrace>\<rho>"
+        by (rule HSem_subset_below[OF cond2' fresh])
+      also have "\<lbrace>\<Delta> @ \<Gamma>\<rbrace>\<rho> = \<lbrace>\<Gamma> @ \<Delta>\<rbrace>\<rho>"
+        by (rule HSem_reorder[OF distinct1 distinct2], auto)
+      finally
+      show "(\<lbrace>\<Delta>\<rbrace>\<rho>)\<^bsub>[fdom (\<lbrace>\<Delta>\<rbrace>\<rho>) \<union> heapVars \<Gamma>]\<^esub> \<sqsubseteq> \<lbrace>\<Gamma> @ \<Delta>\<rbrace>\<rho>"
+        by simp
+      
+    case (goal2 x)[simp]
+      have "ESem (the (map_of \<Gamma> x)) (\<lbrace>\<Gamma> @ \<Delta>\<rbrace>\<rho>) = ESem (the (map_of (\<Gamma>@\<Delta>) x)) (\<lbrace>\<Gamma> @ \<Delta>\<rbrace>\<rho>)"
+        by (simp add: map_add_dom_app_simps)
+      also have "\<dots> \<sqsubseteq> \<lbrace>\<Gamma> @ \<Delta>\<rbrace>\<rho> f! x"
+        by (rule HSem_heap_below[OF cond2], simp)
+      finally
+      show ?case.
+    qed
+  
+    show "\<lbrace>\<Gamma>@\<Delta>\<rbrace>\<rho> \<sqsubseteq> \<lbrace>\<Gamma>\<rbrace>\<lbrace>\<Delta>\<rbrace>\<rho>"
+    proof(rule HSem_below)
+      have "\<rho>\<^bsub>[fdom \<rho> \<union> heapVars (\<Gamma> @ \<Delta>)]\<^esub> = (\<rho>\<^bsub>[fdom \<rho> \<union> heapVars \<Delta>]\<^esub>)\<^bsub>[fdom \<rho> \<union> heapVars (\<Gamma> @ \<Delta>)]\<^esub>"
+        by (rule fmap_expand_idem[symmetric], auto)
+      also have "... \<sqsubseteq> (\<lbrace>\<Delta>\<rbrace>\<rho>)\<^bsub>[fdom \<rho> \<union> heapVars (\<Gamma> @ \<Delta>)]\<^esub>"
+        by (rule cont2monofunE[OF fmap_expand_cont HSem_refines[OF cond3]])
+      also have "... = (\<lbrace>\<Delta>\<rbrace>\<rho>)\<^bsub>[fdom (\<lbrace>\<Delta>\<rbrace>\<rho>) \<union> heapVars (\<Gamma>)]\<^esub>"
+        apply (rule arg_cong) back
+        by auto
+      also have "... \<sqsubseteq> \<lbrace>\<Gamma>\<rbrace>\<lbrace>\<Delta>\<rbrace>\<rho>"
+        by (rule HSem_refines[OF cond1])
+      finally
+      show "\<rho>\<^bsub>[fdom \<rho> \<union> heapVars (\<Gamma> @ \<Delta>)]\<^esub> \<sqsubseteq> \<lbrace>\<Gamma>\<rbrace>\<lbrace>\<Delta>\<rbrace>\<rho> ".
+    
+    case (goal2 x)
+      {
+        assume x[simp]: "x \<in> heapVars \<Gamma>"
+        have "ESem (the (map_of (\<Gamma> @ \<Delta>) x)) (\<lbrace>\<Gamma>\<rbrace>\<lbrace>\<Delta>\<rbrace>\<rho>) = ESem (the (map_of (\<Gamma>) x))(\<lbrace>\<Gamma>\<rbrace>\<lbrace>\<Delta>\<rbrace>\<rho>)"
+          by (simp add: map_add_dom_app_simps)
+        also have "\<dots> \<sqsubseteq> \<lbrace>\<Gamma>\<rbrace>\<lbrace>\<Delta>\<rbrace>\<rho> f! x"
+          by (rule HSem_heap_below[OF cond1 x])
+        finally have ?case.
+      }
+      moreover
+      {
+        assume [simp]:"x \<notin> heapVars \<Gamma>" and  "x \<in> heapVars \<Delta>"
+        have "ESem (the (map_of (\<Gamma> @ \<Delta>) x)) (\<lbrace>\<Gamma>\<rbrace>\<lbrace>\<Delta>\<rbrace>\<rho>) = ESem (the (map_of \<Delta> x)) (\<lbrace>\<Gamma>\<rbrace>\<lbrace>\<Delta>\<rbrace>\<rho>)"
+          by (simp add: map_add_dom_app_simps)
+        also have "\<dots>  = ESem (the (map_of \<Delta> x)) (\<lbrace>\<Delta>\<rbrace>\<rho>)"
+          apply (rule ESem_ignores_fresh[symmetric])
+          apply (rule HSem_disjoint_less)
+            using Gamma_fresh apply auto[1]
+          apply (simp add: fdoms)
+            using fresh apply (metis fresh fresh_PairD(1) fresh_heap_expr'[OF _ the_map_of_snd[OF `x \<in> heapVars \<Delta>`]] fresh_star_def)
+          done
+        also have "\<dots> \<sqsubseteq> \<lbrace>\<Delta>\<rbrace>\<rho> f! x"
+          by (rule HSem_heap_below[OF cond3 `x \<in> heapVars \<Delta>`])
+        also have "\<dots> = \<lbrace>\<Gamma>\<rbrace>\<lbrace>\<Delta>\<rbrace>\<rho> f! x"
+          by (rule the_lookup_HSem_other[symmetric, OF `x \<notin> heapVars \<Gamma>`])
+        finally have ?case.
+      }
+      ultimately show ?case using goal2 by auto
+    qed
+  qed
+
 end
 
 lemma parallel_HSem_ind_different_ESem:
@@ -1008,5 +1159,7 @@ case False
    apply rule
    done
 qed
+
+
 
 end
